03Debruijn/BigStep.thy
@@ -2,60 +2,79 @@ theory BigStep
   imports Termination
 begin
 
-inductive big_evald :: "expr\<^sub>d \<Rightarrow> expr\<^sub>d \<Rightarrow> bool" (infix "\<Down>\<^sub>d" 50) where
-  bevd_const [simp]: "Const\<^sub>d k \<Down>\<^sub>d Const\<^sub>d k"
-| bevd_lam [simp]: "Lam\<^sub>d t e \<Down>\<^sub>d Lam\<^sub>d t e"
-| bevd_app [simp]: "e\<^sub>1 \<Down>\<^sub>d Lam\<^sub>d t e\<^sub>1' \<Longrightarrow> e\<^sub>2 \<Down>\<^sub>d v\<^sub>2 \<Longrightarrow> subst\<^sub>d 0 v\<^sub>2 e\<^sub>1' \<Down>\<^sub>d v \<Longrightarrow> App\<^sub>d e\<^sub>1 e\<^sub>2 \<Down>\<^sub>d v"
+subsection \<open>Big-step evaluation\<close>
+
+text \<open>Now that termination of well-typed expressions is proven, the big-step semantics are easy. We 
+could simply define it as iterated small-step evaluation, but it's easier in the long run to define 
+it analogously to the evaluation of our previous stage (since we subsequently need to prove the 
+equivalence of evaluation across name-removal, and keeping the evaluation relations similar greatly 
+helps with that) and prove the equivalence to small-step evaluation directly.\<close>
+
+inductive big_eval\<^sub>d :: "expr\<^sub>d \<Rightarrow> expr\<^sub>d \<Rightarrow> bool" (infix "\<Down>\<^sub>d" 50) where
+  bev\<^sub>d_const [simp]: "Const\<^sub>d n \<Down>\<^sub>d Const\<^sub>d n"
+| bev\<^sub>d_lam [simp]: "Lam\<^sub>d t e \<Down>\<^sub>d Lam\<^sub>d t e"
+| bev\<^sub>d_app [simp]: "e\<^sub>1 \<Down>\<^sub>d Lam\<^sub>d t e\<^sub>1' \<Longrightarrow> e\<^sub>2 \<Down>\<^sub>d v\<^sub>2 \<Longrightarrow> subst\<^sub>d 0 v\<^sub>2 e\<^sub>1' \<Down>\<^sub>d v \<Longrightarrow> App\<^sub>d e\<^sub>1 e\<^sub>2 \<Down>\<^sub>d v"
 
 inductive_cases [elim]: "Var\<^sub>d x \<Down>\<^sub>d v"
-inductive_cases [elim]: "Const\<^sub>d k \<Down>\<^sub>d v"
+inductive_cases [elim]: "Const\<^sub>d n \<Down>\<^sub>d v"
 inductive_cases [elim]: "Lam\<^sub>d t e \<Down>\<^sub>d v"
 inductive_cases [elim]: "App\<^sub>d e\<^sub>1 e\<^sub>2 \<Down>\<^sub>d v"
 
-lemma [simp]: "e \<Down>\<^sub>d v \<Longrightarrow> value\<^sub>d v"
-  by (induction e v rule: big_evald.induct) simp_all
+text \<open>It is no surprise that two of our three standard properties, determinism and preservation, are 
+simple to prove:\<close>
 
-theorem deterministimb: "e \<Down>\<^sub>d v \<Longrightarrow> e \<Down>\<^sub>d v' \<Longrightarrow> v = v'"
-proof (induction e v arbitrary: v' rule: big_evald.induct)
-  case (bevd_const k)
-  thus ?case by (induction "Const\<^sub>d k" v' rule: big_evald.induct) simp_all
-next
-  case (bevd_lam t e)
-  thus ?case by (induction "Lam\<^sub>d t e" v' rule: big_evald.induct) simp_all
-next
-  case (bevd_app e\<^sub>1 t e\<^sub>1' e\<^sub>2 v\<^sub>2 v)
-  from bevd_app(7, 1, 2, 3, 4, 5, 6) show ?case 
-    by (induction "App\<^sub>d e\<^sub>1 e\<^sub>2" v' rule: big_evald.induct) blast+
-qed
+lemma eval\<^sub>d_to_value [simp]: "e \<Down>\<^sub>d v \<Longrightarrow> value\<^sub>d v"
+  by (induction e v rule: big_eval\<^sub>d.induct) simp_all
 
-lemma [simp]: "value\<^sub>d v \<Longrightarrow> v \<Down>\<^sub>d v"
+lemma eval\<^sub>d_of_value [simp]: "value\<^sub>d v \<Longrightarrow> v \<Down>\<^sub>d v"
   by (induction v) simp_all
 
-lemma completeb' [simp]: "e \<leadsto>\<^sub>d e' \<Longrightarrow> e' \<Down>\<^sub>d v \<Longrightarrow> value\<^sub>d v \<Longrightarrow> e \<Down>\<^sub>d v"
+theorem determinism\<^sub>d\<^sub>b: "e \<Down>\<^sub>d v \<Longrightarrow> e \<Down>\<^sub>d v' \<Longrightarrow> v = v'"
+proof (induction e v arbitrary: v' rule: big_eval\<^sub>d.induct)
+  case (bev\<^sub>d_const n)
+  thus ?case by (induction rule: big_eval\<^sub>d.cases) simp_all
+next
+  case (bev\<^sub>d_lam t e)
+  thus ?case by (induction rule: big_eval\<^sub>d.cases) simp_all
+next
+  case (bev\<^sub>d_app e\<^sub>1 t e\<^sub>1' e\<^sub>2 v\<^sub>2 v)
+  from bev\<^sub>d_app(7, 1, 2, 3, 4, 5, 6) show ?case by (induction rule: big_eval\<^sub>d.cases) blast+
+qed
+
+theorem preservation\<^sub>d\<^sub>b: "e \<Down>\<^sub>d v \<Longrightarrow> \<Gamma> \<turnstile>\<^sub>d e : t \<Longrightarrow> \<Gamma> \<turnstile>\<^sub>d v : t"
+  by (induction e v arbitrary: t rule: big_eval\<^sub>d.induct) fastforce+
+
+text \<open>Now, the correctness and completeness properties: every sequence of iterated small-steps 
+ending in a value is equivalent to a big-step, and vice versa.\<close>
+
+lemma complete\<^sub>d\<^sub>b' [simp]: "e \<leadsto>\<^sub>d e' \<Longrightarrow> e' \<Down>\<^sub>d v \<Longrightarrow> value\<^sub>d v \<Longrightarrow> e \<Down>\<^sub>d v"
 proof (induction e e' arbitrary: v rule: eval\<^sub>d.induct)
   case (ev\<^sub>d_app3 e\<^sub>2 t e\<^sub>1)
   moreover hence "e\<^sub>2 \<Down>\<^sub>d e\<^sub>2" by simp
-  ultimately show ?case by (metis bevd_lam bevd_app)
+  ultimately show ?case by (metis bev\<^sub>d_lam bev\<^sub>d_app)
 qed fastforce+
 
-theorem completeb [simp]: "iter (\<leadsto>\<^sub>d) e v \<Longrightarrow> value\<^sub>d v \<Longrightarrow> e \<Down>\<^sub>d v"
+theorem complete\<^sub>d\<^sub>b [simp]: "iter (\<leadsto>\<^sub>d) e v \<Longrightarrow> value\<^sub>d v \<Longrightarrow> e \<Down>\<^sub>d v"
   by (induction e v rule: iter.induct) simp_all
 
-theorem progressb [simp]: "[] \<turnstile>\<^sub>d e : t \<Longrightarrow> \<exists>v. value\<^sub>d v \<and> e \<Down>\<^sub>d v"
+theorem correct\<^sub>d\<^sub>b: "e \<Down>\<^sub>d v \<Longrightarrow> iter (\<leadsto>\<^sub>d) e v"
+proof (induction e v rule: big_eval\<^sub>d.induct)
+  case (bev\<^sub>d_app e\<^sub>1 t e\<^sub>1' e\<^sub>2 v\<^sub>2 v)
+  hence "iter (\<leadsto>\<^sub>d) (App\<^sub>d e\<^sub>1 e\<^sub>2) (App\<^sub>d (Lam\<^sub>d t e\<^sub>1') e\<^sub>2)" by simp
+  moreover from bev\<^sub>d_app have "iter (\<leadsto>\<^sub>d) (App\<^sub>d (Lam\<^sub>d t e\<^sub>1') e\<^sub>2) (App\<^sub>d (Lam\<^sub>d t e\<^sub>1') v\<^sub>2)" by simp
+  moreover from bev\<^sub>d_app have "App\<^sub>d (Lam\<^sub>d t e\<^sub>1') v\<^sub>2 \<leadsto>\<^sub>d subst\<^sub>d 0 v\<^sub>2 e\<^sub>1'" by simp
+  moreover from bev\<^sub>d_app have "iter (\<leadsto>\<^sub>d) (subst\<^sub>d 0 v\<^sub>2 e\<^sub>1') v" by simp
+  ultimately show ?case by (metis iter_append iter_step)
+qed simp_all
+
+text \<open>Having proved completeness, progress for big-step evaluation is now a simple consequence of 
+the termination theorem.\<close>
+
+theorem progress\<^sub>d\<^sub>b [simp]: "[] \<turnstile>\<^sub>d e : t \<Longrightarrow> \<exists>v. value\<^sub>d v \<and> e \<Down>\<^sub>d v"
 proof -
   assume "[] \<turnstile>\<^sub>d e : t"
   then obtain v where "value\<^sub>d v \<and> iter (\<leadsto>\<^sub>d) e v" by fastforce
   thus ?thesis by fastforce
 qed
-
-theorem correctb: "e \<Down>\<^sub>d v \<Longrightarrow> iter (\<leadsto>\<^sub>d) e v"
-proof (induction e v rule: big_evald.induct)
-  case (bevd_app e\<^sub>1 t e\<^sub>1' e\<^sub>2 v\<^sub>2 v)
-  hence "iter (\<leadsto>\<^sub>d) (App\<^sub>d e\<^sub>1 e\<^sub>2) (App\<^sub>d (Lam\<^sub>d t e\<^sub>1') e\<^sub>2)" by simp
-  moreover from bevd_app have "iter (\<leadsto>\<^sub>d) (App\<^sub>d (Lam\<^sub>d t e\<^sub>1') e\<^sub>2) (App\<^sub>d (Lam\<^sub>d t e\<^sub>1') v\<^sub>2)" by simp
-  moreover from bevd_app have "App\<^sub>d (Lam\<^sub>d t e\<^sub>1') v\<^sub>2 \<leadsto>\<^sub>d subst\<^sub>d 0 v\<^sub>2 e\<^sub>1'" by simp
-  moreover from bevd_app have "iter (\<leadsto>\<^sub>d) (subst\<^sub>d 0 v\<^sub>2 e\<^sub>1') v" by simp
-  ultimately show ?case by (metis iter_append iter_step)
-qed simp_all
 
 end
