03Debruijn/Termination.thy
@@ -1,104 +1,44 @@
 theory Termination
-  imports Multisubst
+  imports Multisubst "../00Utils/Iteration"
 begin
 
-abbreviation terminatesd :: "expr\<^sub>d \<Rightarrow> bool" where
-  "terminatesd e \<equiv> (\<exists>e'. value\<^sub>d e' \<and> iter (\<leadsto>\<^sub>d) e e')"
+subsection \<open>Termination\<close>
 
-primrec stable :: "ty \<Rightarrow> expr\<^sub>d \<Rightarrow> bool" where
-  "stable Num e = (terminatesd e \<and> [] \<turnstile>\<^sub>d e : Num)"
-| "stable (Arrow t\<^sub>1 t\<^sub>2) e = (terminatesd e \<and> ([] \<turnstile>\<^sub>d e : Arrow t\<^sub>1 t\<^sub>2) \<and> 
-    (\<forall>e'. stable t\<^sub>1 e' \<longrightarrow> value\<^sub>d e' \<longrightarrow> stable t\<^sub>2 (App\<^sub>d e e')))"
+text \<open>We are now ready to prove termination of our language. An expression terminates if there is 
+some value that iterated small-step evaluation takes it to. (The \<open>val_no_eval\<^sub>d\<close> lemma ensures that 
+there are no further evaluation steps once a value is reached.)\<close>
 
-lemma stable_typechecks: "stable t e \<Longrightarrow> [] \<turnstile>\<^sub>d e : t"
-  by (induction t) simp_all
+abbreviation terminating :: "expr\<^sub>d \<Rightarrow> bool" where
+  "terminating e \<equiv> (\<exists>v. value\<^sub>d v \<and> iter (\<leadsto>\<^sub>d) e v)"
 
-lemma stable_terminates: "stable t e \<Longrightarrow> terminatesd e"
-  by (induction t) simp_all
-
-lemma [simp]: "terminatesd (Const\<^sub>d k)"
+lemma const_terminates [simp]: "terminating (Const\<^sub>d n)"
 proof
-  show "value\<^sub>d (Const\<^sub>d k) \<and> iter (\<leadsto>\<^sub>d) (Const\<^sub>d k) (Const\<^sub>d k)" by simp
+  show "value\<^sub>d (Const\<^sub>d n) \<and> iter (\<leadsto>\<^sub>d) (Const\<^sub>d n) (Const\<^sub>d n)" by simp
 qed
 
-lemma [simp]: "terminatesd (Lam\<^sub>d t e)"
+lemma lam_terminates [simp]: "terminating (Lam\<^sub>d t e)"
 proof
   show "value\<^sub>d (Lam\<^sub>d t e) \<and> iter (\<leadsto>\<^sub>d) (Lam\<^sub>d t e) (Lam\<^sub>d t e)" by simp
 qed
 
-lemma [simp]: "stable t e \<Longrightarrow> stable t (multisubst es e)"
-proof (induction es)
-  case (Cons e' es)
-  hence "[] \<turnstile>\<^sub>d e : t" by (metis stable_typechecks)
-  hence "subst\<^sub>d 0 e' e = e" by simp
-  with Cons show ?case by simp
-qed simp_all
-
-lemma [simp]: "tc_expr_context \<Gamma> es \<Longrightarrow> list_all2 stable \<Gamma> es \<Longrightarrow> lookup \<Gamma> x = Some t \<Longrightarrow> 
-  stable t (multisubst es (Var\<^sub>d x))"
-proof (induction \<Gamma> es arbitrary: x rule: tc_expr_context.induct)
-  case (tcp_cons t' e \<Gamma> ves)
-  thus ?case by (induction x) simp_all
-qed simp_all
-
-lemma evald_backwards: "iter (\<leadsto>\<^sub>d) e v \<Longrightarrow> value\<^sub>d v \<Longrightarrow> e \<leadsto>\<^sub>d e' \<Longrightarrow> iter (\<leadsto>\<^sub>d) e' v"
+lemma eval\<^sub>d_backwards: "iter (\<leadsto>\<^sub>d) e v \<Longrightarrow> value\<^sub>d v \<Longrightarrow> e \<leadsto>\<^sub>d e' \<Longrightarrow> iter (\<leadsto>\<^sub>d) e' v"
   by (induction e v rule: iter.induct) (metis val_no_eval\<^sub>d, metis determinism\<^sub>d)
 
-lemma [simp]: "e \<leadsto>\<^sub>d e' \<Longrightarrow> terminatesd e = terminatesd e'"
+lemma eval\<^sub>d_terminates [simp]: "e \<leadsto>\<^sub>d e' \<Longrightarrow> terminating e = terminating e'"
 proof 
-  assume "terminatesd e"
+  assume "terminating e"
   then obtain v where V: "value\<^sub>d v \<and> iter (\<leadsto>\<^sub>d) e v" by fastforce
   moreover assume "e \<leadsto>\<^sub>d e'"
-  ultimately have "value\<^sub>d v \<and> iter (\<leadsto>\<^sub>d) e' v" by (metis evald_backwards)
-  thus "terminatesd e'" by fastforce
+  ultimately have "value\<^sub>d v \<and> iter (\<leadsto>\<^sub>d) e' v" by (metis eval\<^sub>d_backwards)
+  thus "terminating e'" by fastforce
 next
-  assume "terminatesd e'"
+  assume "terminating e'"
   then obtain v where V: "value\<^sub>d v \<and> iter (\<leadsto>\<^sub>d) e' v" by fastforce
   moreover assume "e \<leadsto>\<^sub>d e'"
   ultimately have "value\<^sub>d v \<and> iter (\<leadsto>\<^sub>d) e v" by (metis iter_step)
-  thus "terminatesd e" by fastforce
+  thus "terminating e" by fastforce
 qed
 
-lemma stable_evald: "e \<leadsto>\<^sub>d e' \<Longrightarrow> stable t e \<Longrightarrow> stable t e'"
-proof (induction t arbitrary: e e')
-  case (Arrow t\<^sub>1 t\<^sub>2)
-  moreover have "\<And>e\<^sub>2. stable t\<^sub>1 e\<^sub>2 \<Longrightarrow> value\<^sub>d e\<^sub>2 \<Longrightarrow> stable t\<^sub>2 (App\<^sub>d e' e\<^sub>2)" 
-  proof -
-    fix e\<^sub>2
-    assume "stable t\<^sub>1 e\<^sub>2" and "value\<^sub>d e\<^sub>2"
-    with Arrow have X: "stable t\<^sub>2 (App\<^sub>d e e\<^sub>2)" by simp
-    from Arrow have "App\<^sub>d e e\<^sub>2 \<leadsto>\<^sub>d App\<^sub>d e' e\<^sub>2" by simp
-    with Arrow(2) X show "stable t\<^sub>2 (App\<^sub>d e' e\<^sub>2)" by simp
-  qed 
-  ultimately show ?case by simp
-qed simp_all
-
-lemma stable_persists: "iter (\<leadsto>\<^sub>d) e e' \<Longrightarrow> stable t e \<Longrightarrow> stable t e'"
-  by (induction e e' rule: iter.induct) (simp_all add: stable_evald)
-
-lemma stable_evald_back: "[] \<turnstile>\<^sub>d e : t \<Longrightarrow> e \<leadsto>\<^sub>d e' \<Longrightarrow> stable t e' \<Longrightarrow> stable t e"
-proof (induction t arbitrary: e e')
-  case (Arrow t\<^sub>1 t\<^sub>2)
-  from Arrow have "terminatesd e'" by simp
-  with Arrow have X: "terminatesd e" by fastforce
-  have "\<And>e\<^sub>2. stable t\<^sub>1 e\<^sub>2 \<Longrightarrow> value\<^sub>d e\<^sub>2 \<Longrightarrow> stable t\<^sub>2 (App\<^sub>d e e\<^sub>2)" 
-  proof -
-    fix e\<^sub>2
-    assume S: "stable t\<^sub>1 e\<^sub>2" and "value\<^sub>d e\<^sub>2"
-    with Arrow have Y: "stable t\<^sub>2 (App\<^sub>d e' e\<^sub>2)" by simp
-    from S have "[] \<turnstile>\<^sub>d e\<^sub>2 : t\<^sub>1"  by (metis stable_typechecks)
-    with Arrow(3) have Z: "[] \<turnstile>\<^sub>d App\<^sub>d e e\<^sub>2 : t\<^sub>2" by simp
-    from Arrow have "App\<^sub>d e e\<^sub>2 \<leadsto>\<^sub>d App\<^sub>d e' e\<^sub>2" by simp
-    with Arrow Y Z show "stable t\<^sub>2 (App\<^sub>d e e\<^sub>2)" by blast
-  qed
-  with Arrow X show ?case by simp
-qed simp_all
-
-lemma stable_persists_back: "iter (\<leadsto>\<^sub>d) e e' \<Longrightarrow> [] \<turnstile>\<^sub>d e : t \<Longrightarrow> stable t e' \<Longrightarrow> stable t e"
-proof (induction e e' rule: iter.induct)
-  case (iter_step e e' e'')
-  thus ?case using stable_evald_back by fastforce
-qed simp_all
 
 lemma eval_under_app_fst [simp]: "iter (\<leadsto>\<^sub>d) e\<^sub>1 e\<^sub>1' \<Longrightarrow> iter (\<leadsto>\<^sub>d) (App\<^sub>d e\<^sub>1 e\<^sub>2) (App\<^sub>d e\<^sub>1' e\<^sub>2)"
 proof (induction e\<^sub>1 e\<^sub>1' rule: iter.induct)
@@ -117,7 +57,78 @@ proof (induction e\<^sub>2 e\<^sub>2' rule: iter.induct)
   ultimately show ?case by simp
 qed simp_all
 
-lemma tc_stable [simp]: "\<Gamma> \<turnstile>\<^sub>d e : t \<Longrightarrow> tc_expr_context \<Gamma> es \<Longrightarrow> list_all2 stable \<Gamma> es \<Longrightarrow> 
+text \<open>Just proving termination by induction over expressions, or even over typing derivations, fails
+because knowing that \<open>e\<^sub>1\<close> and \<open>e\<^sub>2\<close> terminate tells us nothing about whether \<open>App\<^sub>d e\<^sub>1 e\<^sub>2\<close> terminates; 
+The substitution of \<open>e\<^sub>2\<close> into \<open>e\<^sub>1\<close> can replicate the former to an arbitrary degree. Following Pierce 
+[5], we instead prove a stronger property. We define a "stability" property that says an expression 
+is well-typed and terminating, and also that function-typed stable expressions remain stable when 
+applied to stable arguments. We then prove that every well-typed expression is stable; since all 
+stable expressions terminate, all well-typed expressions are terminating.\<close>
+
+primrec stable :: "ty \<Rightarrow> expr\<^sub>d \<Rightarrow> bool" where
+  "stable Num e = (terminating e \<and> [] \<turnstile>\<^sub>d e : Num)"
+| "stable (Arrow t\<^sub>1 t\<^sub>2) e = (terminating e \<and> ([] \<turnstile>\<^sub>d e : Arrow t\<^sub>1 t\<^sub>2) \<and> 
+    (\<forall>e'. stable t\<^sub>1 e' \<longrightarrow> value\<^sub>d e' \<longrightarrow> stable t\<^sub>2 (App\<^sub>d e e')))"
+
+lemma stable_typechecks: "stable t e \<Longrightarrow> [] \<turnstile>\<^sub>d e : t"
+  by (induction t) simp_all
+
+lemma stable_terminates: "stable t e \<Longrightarrow> terminating e"
+  by (induction t) simp_all
+
+lemma multisubst_var_stable [simp]: "tc_expr_context \<Gamma> es \<Longrightarrow> list_all2 stable \<Gamma> es \<Longrightarrow> 
+  lookup \<Gamma> x = Some t \<Longrightarrow> stable t (multisubst es (Var\<^sub>d x))"
+proof (induction \<Gamma> es arbitrary: x rule: tc_expr_context.induct)
+  case (tcp_cons t' e \<Gamma> ves)
+  thus ?case by (cases x) simp_all
+qed simp_all
+
+lemma stable_eval\<^sub>d: "e \<leadsto>\<^sub>d e' \<Longrightarrow> stable t e \<Longrightarrow> stable t e'"
+proof (induction t arbitrary: e e')
+  case (Arrow t\<^sub>1 t\<^sub>2)
+  moreover have "\<And>e\<^sub>2. stable t\<^sub>1 e\<^sub>2 \<Longrightarrow> value\<^sub>d e\<^sub>2 \<Longrightarrow> stable t\<^sub>2 (App\<^sub>d e' e\<^sub>2)" 
+  proof -
+    fix e\<^sub>2
+    assume "stable t\<^sub>1 e\<^sub>2" and "value\<^sub>d e\<^sub>2"
+    with Arrow have X: "stable t\<^sub>2 (App\<^sub>d e e\<^sub>2)" by simp
+    from Arrow have "App\<^sub>d e e\<^sub>2 \<leadsto>\<^sub>d App\<^sub>d e' e\<^sub>2" by simp
+    with Arrow(2) X show "stable t\<^sub>2 (App\<^sub>d e' e\<^sub>2)" by simp
+  qed 
+  ultimately show ?case by simp
+qed simp_all
+
+lemma stable_persists: "iter (\<leadsto>\<^sub>d) e e' \<Longrightarrow> stable t e \<Longrightarrow> stable t e'"
+  by (induction e e' rule: iter.induct) (simp_all add: stable_eval\<^sub>d)
+
+lemma stable_eval\<^sub>d_back: "[] \<turnstile>\<^sub>d e : t \<Longrightarrow> e \<leadsto>\<^sub>d e' \<Longrightarrow> stable t e' \<Longrightarrow> stable t e"
+proof (induction t arbitrary: e e')
+  case (Arrow t\<^sub>1 t\<^sub>2)
+  from Arrow have "terminating e'" by simp
+  with Arrow have X: "terminating e" by fastforce
+  have "\<And>e\<^sub>2. stable t\<^sub>1 e\<^sub>2 \<Longrightarrow> value\<^sub>d e\<^sub>2 \<Longrightarrow> stable t\<^sub>2 (App\<^sub>d e e\<^sub>2)" 
+  proof -
+    fix e\<^sub>2
+    assume S: "stable t\<^sub>1 e\<^sub>2" and "value\<^sub>d e\<^sub>2"
+    with Arrow have Y: "stable t\<^sub>2 (App\<^sub>d e' e\<^sub>2)" by simp
+    from S have "[] \<turnstile>\<^sub>d e\<^sub>2 : t\<^sub>1"  by (metis stable_typechecks)
+    with Arrow(3) have Z: "[] \<turnstile>\<^sub>d App\<^sub>d e e\<^sub>2 : t\<^sub>2" by simp
+    from Arrow have "App\<^sub>d e e\<^sub>2 \<leadsto>\<^sub>d App\<^sub>d e' e\<^sub>2" by simp
+    with Arrow Y Z show "stable t\<^sub>2 (App\<^sub>d e e\<^sub>2)" by blast
+  qed
+  with Arrow X show ?case by simp
+qed simp_all
+
+lemma stable_persists_back: "iter (\<leadsto>\<^sub>d) e e' \<Longrightarrow> [] \<turnstile>\<^sub>d e : t \<Longrightarrow> stable t e' \<Longrightarrow> stable t e"
+proof (induction e e' rule: iter.induct)
+  case (iter_step e e' e'')
+  thus ?case using stable_eval\<^sub>d_back by fastforce
+qed simp_all
+
+text \<open>We prove the crucial lemma about \<open>multisubst\<close> rather than \<open>subst\<^sub>d\<close> because stability is only 
+defined over closed expressions, and we need to substitute for all free variables in an arbitrary 
+expression at once to get a closed term.\<close>
+
+lemma tc_stable_multisubst [simp]: "\<Gamma> \<turnstile>\<^sub>d e : t \<Longrightarrow> tc_expr_context \<Gamma> es \<Longrightarrow> list_all2 stable \<Gamma> es \<Longrightarrow> 
   stable t (multisubst es e)"
 proof (induction \<Gamma> e t arbitrary: es rule: typing\<^sub>d.induct)
   case (tc\<^sub>d_lam t\<^sub>1 \<Gamma> e t\<^sub>2)
@@ -138,15 +149,15 @@ proof (induction \<Gamma> e t arbitrary: es rule: typing\<^sub>d.induct)
     moreover with V have "App\<^sub>d (Lam\<^sub>d t\<^sub>1 e') e\<^sub>2 \<leadsto>\<^sub>d subst\<^sub>d 0 e\<^sub>2 e'" by simp
     moreover from E have "[] \<turnstile>\<^sub>d Lam\<^sub>d t\<^sub>1 e' : Arrow t\<^sub>1 t\<^sub>2" by simp
     moreover with E2 have "[] \<turnstile>\<^sub>d App\<^sub>d (Lam\<^sub>d t\<^sub>1 e') e\<^sub>2 : t\<^sub>2" by simp
-    ultimately show "stable t\<^sub>2 (App\<^sub>d (Lam\<^sub>d t\<^sub>1 e') e\<^sub>2)" by (metis stable_evald_back)
+    ultimately show "stable t\<^sub>2 (App\<^sub>d (Lam\<^sub>d t\<^sub>1 e') e\<^sub>2)" by (metis stable_eval\<^sub>d_back)
   qed
   ultimately show ?case by simp
 next
   case (tc\<^sub>d_app \<Gamma> e\<^sub>1 t\<^sub>1 t\<^sub>2 e\<^sub>2)
-  hence "terminatesd (multisubst es e\<^sub>2)" by (metis stable_terminates)
+  hence "terminating (multisubst es e\<^sub>2)" by (metis stable_terminates)
   then obtain v\<^sub>2 where V2: "value\<^sub>d v\<^sub>2 \<and> iter (\<leadsto>\<^sub>d) (multisubst es e\<^sub>2) v\<^sub>2" by fastforce
   with tc\<^sub>d_app have V2S: "stable t\<^sub>1 v\<^sub>2" by (metis stable_persists)
-  from tc\<^sub>d_app have "terminatesd (multisubst es e\<^sub>1)" by fastforce
+  from tc\<^sub>d_app have "terminating (multisubst es e\<^sub>1)" by fastforce
   then obtain v\<^sub>1 where V1: "value\<^sub>d v\<^sub>1 \<and> iter (\<leadsto>\<^sub>d) (multisubst es e\<^sub>1) v\<^sub>1" by fastforce
   with tc\<^sub>d_app have SV: "stable (Arrow t\<^sub>1 t\<^sub>2) v\<^sub>1" by (metis stable_persists)
   with V2S V2 have "stable t\<^sub>2 (App\<^sub>d v\<^sub>1 v\<^sub>2)" by simp
@@ -164,11 +175,12 @@ next
   thus ?case by simp
 qed simp_all
 
-theorem tc_terminationd [simp]: "[] \<turnstile>\<^sub>d e : t \<Longrightarrow> terminatesd e"
+theorem tc_terminationd [simp]: "[] \<turnstile>\<^sub>d e : t \<Longrightarrow> terminating e"
 proof -
   assume "[] \<turnstile>\<^sub>d e : t" 
   moreover have "list_all2 stable [] []" by simp
-  ultimately show ?thesis by (metis stable_terminates multisubst.simps(1) tcp_nil tc_stable)
+  ultimately show ?thesis 
+    by (metis stable_terminates multisubst.simps(1) tcp_nil tc_stable_multisubst)
 qed
 
 end
